extended bucket sort

sv_boogie.bpl
@@ -4,7 +4,7 @@ axiom 0 <= N;
 
 // Declare a map from integers to integers.
 // 'a' should be treated as an array of 'N' elements, indexed from 0 to N-1
-var a: [int]int;
+var a, b0, b1, b2: [int]int;
 
 // Returns true iff the elements of 'arr' are small (i.e. values in the range -3N to +3N)
 function has_small_elements(arr: [int]int): bool
@@ -14,7 +14,7 @@ function has_small_elements(arr: [int]int): bool
 
 // Sorts 'a' using bucket sort or quick sort, as determined by has_small_elements(a)
 procedure sort() returns (perm : [int]int)
-  modifies a;
+  modifies a,b0,b1,b2;
   // perm is a permutation
   ensures (forall i: int :: 0 <= i && i <= N-1 ==> 0 <= perm[i] && perm[i] <= N-1);
   ensures (forall k, l: int :: 0 <= k && k < l && l <= N-1 ==> perm[k] != perm[l]);
@@ -38,7 +38,7 @@ procedure sort() returns (perm : [int]int)
  
 }
 
-
+/*
 
 procedure qsPartition(lo : int, hi : int) returns (pivot_index: int, perm: [int]int) 
   modifies a;
@@ -182,10 +182,91 @@ procedure qs(lo : int, hi : int) returns (perm: [int]int)
     
 }
 
-procedure bs(lo : int, hi : int) returns (perm: [int]int)
+*/
+
+
+// dummy sort implementation for faster development times
+procedure qs(lo : int, hi : int) returns (perm: [int]int) 
   modifies a;
   requires lo <= hi;
+  
+  // perm is a permutation
+  ensures (forall i: int :: lo <= i && i <= hi ==> lo <= perm[i] && perm[i] <= hi);
+  ensures (forall k, l: int :: lo <= k && k < l && l <= hi ==> perm[k] != perm[l]);
+  // the final array is that permutation of the input array
+  ensures (forall i: int :: lo <= i && i <= hi ==> a[i] == old(a)[perm[i]]);
+  // array is sorted
+  ensures (forall k, l: int :: lo <= k && k <= l && l <= hi ==> a[k] <= a[l]);
+  // rest of the array is untouched
+  ensures (forall k: int :: k < lo || k > hi ==> a[k] == old(a)[k]);
+{
+ // perm is a permutation
+  assume (forall i: int :: lo <= i && i <= hi ==> lo <= perm[i] && perm[i] <= hi);
+  assume (forall k, l: int :: lo <= k && k < l && l <= hi ==> perm[k] != perm[l]);
+  // the final array is that permutation of the input array
+  assume (forall i: int :: lo <= i && i <= hi ==> a[i] == old(a)[perm[i]]);
+  // array is sorted
+  assume (forall k, l: int :: lo <= k && k <= l && l <= hi ==> a[k] <= a[l]);
+  // rest of the array is untouched
+  assume (forall k: int :: k < lo || k > hi ==> a[k] == old(a)[k]);  
+}
+
+// dummy sort implementation for faster development times
+procedure qs_b0(lo : int, hi : int) returns (perm: [int]int) 
+  modifies b0;
+  requires lo <= hi;
+  
+  ensures (forall i: int :: lo <= i && i <= hi ==> lo <= perm[i] && perm[i] <= hi);
+  ensures (forall k, l: int :: lo <= k && k < l && l <= hi ==> perm[k] != perm[l]);
+  ensures (forall i: int :: lo <= i && i <= hi ==> b0[i] == old(b0)[perm[i]]);
+  ensures (forall k, l: int :: lo <= k && k <= l && l <= hi ==> b0[k] <= b0[l]);
+  ensures (forall k: int :: k < lo || k > hi ==> b0[k] == old(b0)[k]);
+{
+  assume (forall i: int :: lo <= i && i <= hi ==> lo <= perm[i] && perm[i] <= hi);
+  assume (forall k, l: int :: lo <= k && k < l && l <= hi ==> perm[k] != perm[l]);
+  assume (forall i: int :: lo <= i && i <= hi ==> b0[i] == old(b0)[perm[i]]);
+  assume (forall k, l: int :: lo <= k && k <= l && l <= hi ==> b0[k] <= b0[l]);
+  assume (forall k: int :: k < lo || k > hi ==> b0[k] == old(b0)[k]);  
+}
+procedure qs_b1(lo : int, hi : int) returns (perm: [int]int) 
+  modifies b1;
+  requires lo <= hi;
+  
+  ensures (forall i: int :: lo <= i && i <= hi ==> lo <= perm[i] && perm[i] <= hi);
+  ensures (forall k, l: int :: lo <= k && k < l && l <= hi ==> perm[k] != perm[l]);
+  ensures (forall i: int :: lo <= i && i <= hi ==> b1[i] == old(b1)[perm[i]]);
+  ensures (forall k, l: int :: lo <= k && k <= l && l <= hi ==> b1[k] <= b1[l]);
+  ensures (forall k: int :: k < lo || k > hi ==> b1[k] == old(b1)[k]);
+{
+  assume (forall i: int :: lo <= i && i <= hi ==> lo <= perm[i] && perm[i] <= hi);
+  assume (forall k, l: int :: lo <= k && k < l && l <= hi ==> perm[k] != perm[l]);
+  assume (forall i: int :: lo <= i && i <= hi ==> b1[i] == old(b1)[perm[i]]);
+  assume (forall k, l: int :: lo <= k && k <= l && l <= hi ==> b1[k] <= b1[l]);
+  assume (forall k: int :: k < lo || k > hi ==> b1[k] == old(b1)[k]);  
+}
+procedure qs_b2(lo : int, hi : int) returns (perm: [int]int) 
+  modifies b2;
+  requires lo <= hi;
+  
+  ensures (forall i: int :: lo <= i && i <= hi ==> lo <= perm[i] && perm[i] <= hi);
+  ensures (forall k, l: int :: lo <= k && k < l && l <= hi ==> perm[k] != perm[l]);
+  ensures (forall i: int :: lo <= i && i <= hi ==> b2[i] == old(b2)[perm[i]]);
+  ensures (forall k, l: int :: lo <= k && k <= l && l <= hi ==> b2[k] <= b2[l]);
+  ensures (forall k: int :: k < lo || k > hi ==> b2[k] == old(b2)[k]);
+{
+  assume (forall i: int :: lo <= i && i <= hi ==> lo <= perm[i] && perm[i] <= hi);
+  assume (forall k, l: int :: lo <= k && k < l && l <= hi ==> perm[k] != perm[l]);
+  assume (forall i: int :: lo <= i && i <= hi ==> b2[i] == old(b2)[perm[i]]);
+  assume (forall k, l: int :: lo <= k && k <= l && l <= hi ==> b2[k] <= b2[l]);
+  assume (forall k: int :: k < lo || k > hi ==> b2[k] == old(b2)[k]);  
+}
+
+procedure bs(lo : int, hi : int) returns (perm: [int]int)
+  modifies a, b0, b1, b2;
+  requires lo <= hi;
   requires lo >= 0;
+  // only use bucket sort when these conditions hols
+  requires (forall i: int :: (0 <= i && i < N) ==> (-3 * N <= a[i] && a[i] <= 3 * N));
   
   // perm is a permutation
   ensures (forall i: int :: lo <= i && i <= hi ==> lo <= perm[i] && perm[i] <= hi);
@@ -201,10 +282,10 @@ procedure bs(lo : int, hi : int) returns (perm: [int]int)
 {
   //assumption: all values are within the [-3N, 3N] range where N = length of `a'
   
-  //we're using three buckets:
-  var b0: [int]int; //bucket for values [-3N,-1N)
-  var b1: [int]int; //bucket for values [-1N,1N)
-  var b2: [int]int; //bucket for values [1N,3N]
+  //we're using three buckets: TODO at the moment we're using global arrays
+  //var b0: [int]int; // bucket for values [-3N,-1N)
+  //var b1: [int]int; //bucket for values [-1N,1N)
+  //var b2: [int]int; //bucket for values [1N,3N]
   
   //buckets' start/end indices
   var b0_i:int;
@@ -216,8 +297,11 @@ procedure bs(lo : int, hi : int) returns (perm: [int]int)
   var bound_1:int;
   var bound_2:int;
   
+  //bucket permutations
+  var perm0, perm1, perm2 : [int]int;
+  
   //iterator variables
-  var i,k:int;
+  var i :int;
   
   b0_i := 0;
   b1_i := 0;
@@ -264,39 +348,53 @@ procedure bs(lo : int, hi : int) returns (perm: [int]int)
   //debugging: check all elements have been inserted into a bucket
   assert(forall e:int :: ((e >= lo && e < hi) ==> (exists t:int :: (b0[t] == a[e] || b1[t] == a[e] || b2[t] == a[e]))));
   
-  //sort the buckets
-  //TODO (?): call QS to sort b0 for the range [0..(b0_i - 1)]
-  //TODO (?): call QS to sort b1 for the range [0..(b1_i - 1)]
-  //TODO (?): call QS to sort b2 for the range [0..(b2_i - 1)]
-  assume(forall e:int :: ((e > 0 && e < b0_i) ==> (b0[e-1] <= b0[e])));
-  assume(forall e:int :: ((e > 0 && e < b1_i) ==> (b1[e-1] <= b1[e])));
-  assume(forall e:int :: ((e > 0 && e < b2_i) ==> (b2[e-1] <= b2[e])));
   
   //TODO (?): keep track of permutations
-  
-  i := lo;
-  while(i < b0_i)
-    //TODO: invariants
-    {
-    a[i] := b0[i];
-    i := i + 1;
+    
+  //sort the buckets
+  if(b0_i > 0) { // if bucket is non empty
+      call perm0 := qs_b0(0, b0_i-1);
+      i := 0;
+      while(i < b0_i)
+        invariant (forall k: int :: 0 <= k && k < i ==> a[lo + i] == b0[i]);
+        invariant (forall k, l: int :: lo <= k && k <= l && l < lo + i ==> a[k] <= a[l]);
+        //TODO: invariants
+      {
+        a[lo + i] := b0[i];
+        i := i + 1;
+      }
+      //here the array from lo...lo+bo_i-1 is sorted
+      assert (forall k, l: int :: lo <= k && k <= l && l < lo + b0_i ==> a[k] <= a[l]);
   }
   
-  k := 0;
-  while(k < b1_i)
-    //TODO: invariants
-    {
-    a[i] := b1[k];
-    i := i + 1;
-    k := k + 1;
+  if(b1_i > 0) { // if bucket is non empty
+      call perm1 := qs_b1(0, b1_i-1);
+      i := 0;
+      while(i < b1_i)
+        invariant (forall k: int :: 0 <= k && k < i ==> a[b0_i + i] == b1[i]);
+        invariant (forall k, l: int :: b0_i <= k && k <= l && l < b0_i + i ==> a[k] <= a[l]);
+        //TODO: invariants
+      {
+        a[b0_i + i] := b1[i];
+        i := i + 1;
+      }
+      //here the array from lo...lo+bo_i-1 is sorted
+      assert (forall k, l: int :: b0_i <= k && k <= l && l < b0_i + b1_i ==> a[k] <= a[l]);
+  }
+ 
+   if(b2_i > 0) { // if bucket is non empty
+      call perm2 := qs_b2(0, b2_i-1);
+      i := 0;
+      while(i < b2_i)
+        invariant (forall k: int :: 0 <= k && k < i ==> a[b1_i + i] == b2[i]);
+        invariant (forall k, l: int :: b1_i <= k && k <= l && l < b1_i + i ==> a[k] <= a[l]);
+        //TODO: invariants
+      {
+        a[b1_i + i] := b2[i];
+        i := i + 1;
+      }
+      //here the array from lo...lo+bo_i-1 is sorted
+      assert (forall k, l: int :: b1_i <= k && k <= l && l < b1_i + b2_i ==> a[k] <= a[l]);
   }
   
-  k := 0;
-  while(k < b2_i)
-    //TODO: invariants
-    {
-    a[i] := b2[k];
-    i := i + 1;
-    k := k + 1;
-  }
 }
